apps/tc/theories/tc.v
@@ -209,3 +209,11 @@ Elpi Accumulate File cs.
 Elpi Accumulate lp:{{
   main L :- cs.main L.
 }}.
+
+Elpi Tactic solve_cs.
+Elpi Accumulate Db tc.db.
+Elpi Accumulate File tc_aux.
+Elpi Accumulate File cs.
+(* Elpi Accumulate lp:{{
+  main L :- cs.main L.
+}}. *)
